src/program_proof/mvcc/txn_do_txn.v
@@ -1,0 +1,86 @@
+From Perennial.program_proof.mvcc Require Import mvcc_inv txn_common txn_begin txn_commit.
+
+Section program.
+Context `{!heapGS Σ, !mvcc_ghostG Σ}.
+
+Definition txnmap_ptstos τ (m : dbmap) : iProp Σ :=
+  [∗ map] k ↦ v ∈ m, txnmap_ptsto τ k v.
+
+Definition dbmap_ptstos γ (m : dbmap) : iProp Σ :=
+  [∗ map] k ↦ v ∈ m, dbmap_ptsto γ k v.
+
+Definition spec_body (body : val) (txn :loc) r P Q τ : iProp Σ :=
+  {{{ ⌜P r⌝ ∗ txnmap_ptstos τ r }}}
+    body #txn
+  {{{ w (ok : bool), RET #ok; if ok then ⌜Q r w⌝ ∗ txnmap_ptstos τ w else True }}}.
+
+Theorem wp_txn__DoTxn txn (body : val) P Q γ :
+  (∀ r w, (Decision (Q r w))) ->
+  ⊢ {{{ own_txn_uninit txn γ ∗ (∀ r τ, spec_body body txn r P Q τ) }}}
+    <<< ∀∀ (r : dbmap), ⌜P r⌝ ∗ dbmap_ptstos γ r >>>
+      Txn__DoTxn #txn body @ ↑mvccNSST
+    <<< ∃∃ (ok : bool), if ok then (∃ w, ⌜Q r w⌝ ∗ dbmap_ptstos γ w) else dbmap_ptstos γ r >>>
+    {{{ (v : u64), RET #ok; own_txn_uninit txn γ }}}.
+Proof.
+  iIntros (Hdec) "!>".
+  iIntros (Φ) "[Htxn Hbody] HAU".
+  wp_call.
+
+  (***********************************************************)
+  (* txn.Begin()                                             *)
+  (* cmt := body(txn)                                        *)
+  (* if !cmt {                                               *)
+  (*     txn.Abort()                                         *)
+  (*     return false                                        *)
+  (* }                                                       *)
+  (* txn.Commit()                                            *)
+  (* return true                                             *)
+  (***********************************************************)
+  wp_apply (wp_txn__Begin with "Htxn").
+  iIntros "[%τ Htxn]".
+  wp_pures.
+  wp_apply ("Hbody").
+  { (* TODO: Prove precondition. *) admit. }
+  iIntros (w ok) "H".
+  wp_pures.
+  wp_if_destruct.
+  { (* Abort branch. *) admit. }
+  wp_apply (wp_txn__Commit with "Htxn").
+  iIntros (ok) "Htxn".
+  wp_pures.
+Admitted.
+
+
+Definition pre_Swap (r : dbmap) : Prop.
+Admitted.
+Definition post_Swap (r w : dbmap) : Prop.
+Admitted.
+
+Theorem wp_SwapSeq txn r τ :
+  {{{ ⌜pre_Swap r⌝ ∗ txnmap_ptstos τ r }}}
+    SwapSeq #txn
+  {{{ w (ok : bool), RET #ok; if ok then ⌜post_Swap r w⌝ ∗ txnmap_ptstos τ w else True }}}.
+Admitted.
+
+Instance post_Swap_dec : (∀ r w, (Decision (post_Swap r w))).
+Admitted.
+
+Theorem wp_Swap (txn : loc) γ :
+  ⊢ {{{ own_txn_uninit txn γ }}}
+    <<< ∀∀ (r : dbmap), ⌜pre_Swap r⌝ ∗ dbmap_ptstos γ r >>>
+      Swap #txn @ ↑mvccNSST
+    <<< ∃∃ (ok : bool), if ok then (∃ w, ⌜post_Swap r w⌝ ∗ dbmap_ptstos γ w) else dbmap_ptstos γ r >>>
+    {{{ (v : u64), RET #ok; own_txn_uninit txn γ }}}.
+Proof.
+  iIntros "!>".
+  iIntros (Φ) "Htxn HAU".
+  wp_call.
+  wp_apply (wp_txn__DoTxn _ _ _ post_Swap with "[$Htxn]").
+  { unfold spec_body.
+    iIntros (r τ Φ') "!> Hpre HΦ'".
+    iApply (wp_SwapSeq with "Hpre HΦ'").
+  }
+  done.
+Qed.
+
+End program.
